<section xml:id="Sec_AdvancedDerivative">
  <title>Advanced Derivatve Techniques</title>

  <subsection>
    <title>Product Rule </title>
  <p>
    Since the behavior of derivatives of sums behave so well,
    its tempting to believe that the derivatives of products would behave similarly well, that is,
    it may be reasonable to guess that <m>\frac{d}{dx}[f(x)g(x)]=f'(x)g'(x)</m>.
    To try to see if this is true, we should ask, is:
    <me>
      \frac{d}{dx}[x\cdot x]=\frac{d}{dx}[x]\frac{d}{dx}[x]?
    </me>
  </p>
  <p>
    Well on the left hand side <m>\frac{d}{dx}[x\cdot x]=\frac{d}{dx}[x^2]=2x</m>.
    On the right, <m>\frac{d}{dx}[x]\frac{d}{dx}[x]=1\cdot1=1</m>,
    so these are clearly not the same.  It's safe to say that in general <me> \frac{d}{dx}[f(x)g(x)]\neq f'(x)g'(x).</me>
  </p>
  

    <remark xml:id="ProductRule">
      <statement>
        <p>
    We <em>do</em> have a rule for the derivative of products. The
    <term> product rule</term>
    and it states <m>\frac{d}{dx}[f(x)g(x)]=f'(x)g(x)+f(x)g'(x)</m>.
    To see why:
    <md>
      <mrow>\frac{d}{dx}[f(x)g(x)]\amp = \limit{h}{0}\frac{f(x+h)g(x+h)-f(x)g(x)}{h},\ \text{ at this stage, I'm going to pull a clever trick and add by 0: }</mrow>
      <mrow>\amp = \limit{h}{0}\frac{f(x+h)g(x+h)\color{blue}{-f(x)g(x+h)+f(x)g(x+h)}-f(x)g(x)}{h}</mrow>
      <mrow>\amp = \limit{h}{0}\frac{f(x+h)g(x+h)-f(x)g(x+h)}{h}+\limit{h}{0}\frac{f(x)g(x+h)-f(x)g(x)}{h}</mrow>
      <mrow>\amp = \limit{h}{0}\frac{f(x+h)-f(x)}{h}g(x+h)+\limit{h}{0}f(x)\frac{g(x+h)-g(x)}{h}</mrow>
      <mrow>\amp = f'(x)g(x)+f(x)g'(x)</mrow>
    </md>.
  </p>
</statement>
</remark>

=

<example>
  <title>Applying the Product Rule</title>
  <statement>
    <p>
      Compute the derivative of
      <m>f(x)=x^3(x+1)</m>.
    </p>
  </statement>

<solution>
  <p>
  Utilizing <xref ref="ProductRule" />:
      <md>
        <mrow>f'(x)\amp = \frac{d}{dx}[x^3](x+1)+x^3\frac{d}{dx}[x+1]</mrow>
        <mrow>\amp = 3x^2(x+1)+x^3(1)</mrow>
        <mrow>\amp = 3x^3+3x^2+x^3</mrow>
        <mrow>\amp = 4x^3+3x^2</mrow>
      </md>.
    </p>
    <p>
      Also note we could have computed this some other way:
      <md>
        <mrow>f(x)\amp = x^3(x+1)=x^4+x^3</mrow>
        <mrow>f'(x)\amp = 4x^3+3x^2</mrow>
      </md>.
      We can see this:
      <interactive desmos="wm9bx7pbb6"/>
    </p>
  </solution>
</example>


</subsection>


<subsection>
  <title>Quotient Rule</title>

  <p> It should seem clear that <me>\frac{d}{dx}[\frac{f(x)}{g(x)}]\neq \frac{f'(x)}{g'(x)}.</me></p>

 <remark xml:id="QuotientRule">
      <statement>
        <p>
    We have an analagous rule for the derivative of quotients. The
    <term> quotient rule</term>
    and it states <m>\frac{d}{dx}[\frac{f(x)}{g(x)}]=\frac{f'(x)g(x)-f(x)g'(x)}{g(x)^2}</m>.
    To see why, let <m>Q(x)=\frac{f(x)}{g(x)}</m> and observe:
    <md>
      <mrow>Q(x)\amp = \frac{f(x)}{g(x)}</mrow>
        <mrow>Q(x)g(x)\amp = f(x),\ \text{ now we can differentiate both sides }</mrow>
        <mrow>\frac{d}{dx}[Q(x)g(x)]\amp = f'(x),\ \text{ then by the product rule: }</mrow>
        <mrow>Q'(x)g(x)+Q(x)g'(x)\amp = f'(x)</mrow>
        <mrow>Q'(x)g(x)\amp = f'(x)-Q(x)g'(x),\ \text{then recall that  \(Q(x)=\frac{f(x)}{g(x)}\)}</mrow>
        <mrow>Q'(x)g(x)\amp = f'(x)-\frac{f(x)g'(x)}{g(x)}</mrow>
        <mrow>Q'(x)g(x)\amp = \frac{f'(x)g(x)-f(x)g'(x)}{g(x)}</mrow>
        <mrow>Q'(x)\amp = \frac{f'(x)g(x)-f(x)g'(x)}{g(x)^2}</mrow>
    </md>.
  </p>
</statement>
</remark>


<example>
  <statement>
    <p>
      Compute the derivative of
      <m>g(x)=\frac{x}{x^2+1}</m>.
    </p>
  </statement>

<solution>
  <p>
  Utilizing <xref ref="QuotientRule" />:
      <md>
        <mrow>g'(x)\amp = \frac{(x^2+1)\frac{d}{dx}[x]-x\frac{d}{dx}[x^2+1]}{(x^2+1)^2}</mrow>
        <mrow>\amp = \frac{(x^2+1)(1)-x(2x)}{(x^2+1)^2}</mrow>
        <mrow>\amp = \frac{1-x^2}{(x^2+1)^2}</mrow>
      </md>.
      We can see this:
      <interactive desmos="mznhnfb6m3"/>
    </p>
  </solution>
</example>


</subsection>


<subsection>
  <title>Chain Rule</title>

<p> We finally have a rule for composition of functions:</p>

 <remark xml:id="ChainRule">
      <statement>
        <p>
     The
    <term> chain rule</term>
     states <me>\frac{d}{dx}[f(g(x))]=f'(g(x))g'(x).</me>
    To see why:
    <md>
        <mrow>\frac{d}{dx}[f(g(x))]\amp = \limit{h}{0}\frac{f(g(x+h))-f(g(x))}{h},\ \text{ Similar to the product rule, we will multiply by 1: }</mrow>
        <mrow>\amp = \limit{h}{0}\frac{f(g(x+h))-f(g(x))}{h}\color{blue}{\frac{g(x+h)-g(x)}{g(x+h)-g(x)}}</mrow>
        <mrow>\amp = \limit{h}{0}\frac{f(g(x+h))-f(g(x))}{g(x+h)-g(x)}\frac{g(x+h)-g(x)}{h}</mrow>
        <mrow>\amp = \limit{h}{0}\frac{f(g(x+h))-f(g(x))}{g(x+h)-g(x)}\limit{h}{0}\frac{g(x+h)-g(x)}{h}</mrow>

    </md>.
  </p>

  <p>
      We're going to play a second trick here,
      we are going to let <m>k=g(x+h)-g(x)</m>,
      we also note then that <m>g(x+h+=g(x)+k</m>.
      Also note that when <m>h\to 0</m> It follows that <m>k=g(x+h)-g(x)\to g(x+0)-g(x)=0</m>.
      So we can make some replacements:
      <md>
        <mrow>\amp = \limit{h}{0}\frac{f(g(x+h))-f(g(x))}{g(x+h)-g(x)}\limit{h}{0}\frac{g(x+h)-g(x)}{h}</mrow>
        <mrow>\amp = \limit{\color{red}{k}}{0}\frac{f(\color{red}{g(x)+k})-f(g(x))}{\color{red}{k}}\limit{h}{0}\frac{g(x+h)-g(x)}{h}</mrow>
        <mrow>\amp = f'(g(x))g'(x)</mrow>
      </md>
    </p>
</statement>
</remark>


<example>
  <title>Applying the Chain Rule</title>
  <statement>
    <p>
      Compute the derivative of
      <m>f(x)=\sqrt{x^2+1}</m>.
    </p>
  </statement>

<solution>
  <p>
  We can think of this as <m>f(x)=g(h(x))</m> where <m>g(x)=\sqrt{x}=x^{1/2}, h(x)=x^2+1</m>.
      So <m>g'(x)=\frac{1}{2}x^{-1/2}, h'(x)=2x</m>.  Utilizing <xref ref="ChainRule" />:
     <md>
        <mrow>f'(x)\amp = \frac{d}{dx}[\sqrt{x^2+1}]</mrow>
        <mrow>\amp = \frac{d}{dx}[g(h(x))]</mrow>
        <mrow>\amp = g'(h(x))h'(x)</mrow>
        <mrow>\amp = \frac{1}{2}(x^2+1)^{-1/2}(2x)</mrow>
        <mrow>\amp = \frac{x}{\sqrt{x^2+1}}</mrow>
      </md>.
      We can see this:
      <interactive desmos="ixfpretw0i"/>
    </p>
  </solution>
</example>



</subsection>



<subsection>
  <title>Exercises</title>
<exercise>
  <statement>
    <p>
      The total profit \from selling
<m>x</m> widgets is: <me>P(x)=\$ \frac{200x-1000}{20x+30}.</me>
Find the marginal average cost function.


    </p>
  </statement>

<solution>
  <p>
  If you sell <m>x</m> widgets, the total profit is <m>P(x)=\$ \frac{200x-1000}{20x+30}.</m>  So the average profit per widget is <me>A(x)=\frac{P(x)}{x}= \frac{200x-1000}{20x+30}\cdot\frac{1}{x}=\frac{200x-1000}{20x^2+30x}.</me>  Then, the marginal average cost is computed via the derivative:
     <md>
        <mrow>A'(x)\amp = \frac{d}{dx}[\frac{200x-1000}{20x^2+30x}]</mrow>
        <mrow>\amp = \frac{\frac{d}{dx}[200x-1000](20x^2+30x)-(200x-1000)\frac{d}{dx}[20x^2-30x]}{(20x^2+30x)^2}</mrow>
        <mrow>\amp = \frac{200(20x^2+30x)-(200x-1000)(40x-30)}{(20x^2+30x)^2}</mrow>
        <mrow>\amp = \frac{4000x^2+6000x-(8000x^2-34000x-30000)}{(20x^2+30x)^2}</mrow>
        <mrow>\amp = \frac{4000x^2+6000x-8000x^2+34000x+30000}{(20x^2+30x)^2}</mrow>
        <mrow>\amp = \frac{-4000x^2+40000x+30000}{(20x^2+30x)^2}</mrow>
      </md>.
      We can see this:
      <interactive desmos="fzzio7tkr5"/>
    </p>
  </solution>
</exercise>


<exercise>
  <statement>
    <p>
      Assume that the total number (in millions)
of bacteria present in a culture at a certain time <m>t</m> (in
hours) is given by <me> N(t)=3t(t-8)^2+30.</me>
<ol>
  <li>Find <m>N'(t)</m>.</li>
  <li> How fast is the population of bacteria growing in 10 hours?</li>
</ol>  

    </p>
  </statement>

<solution>
  <p>
    Consider:

    <ol>
  <li>We compute <m>N'(t)</m>:
   <md>
        <mrow>N'(t)\amp = \frac{d}{dt}[3t(t-8)^2+30]</mrow>
        <mrow>\amp = \frac{d}{dt}[3t(t-8)^2]+\frac{d}{dt}[30]</mrow>
        <mrow>\amp = \frac{d}{dt}[3t](t-8)^2+3t\frac{d}{dt}[(t-8)^2]+0</mrow>
        <mrow>\amp = 3(t-8)^2+3t\frac{d}{dt}[t^2-16t+64]</mrow>
        <mrow>\amp = 3(t^2-16t+64)+3t(2t-16))</mrow>
         <mrow>\amp = 3t^2-48t+192+6t^2-48t</mrow>
         <mrow>\amp = 9t^2-96t+192</mrow>
      </md>.
</li>
  <li> Notice that <m>N(10)=9(10^2)-96(10)+192=132</m> or 132 million bacteria per hour.</li>
</ol>  

  
      We can see this:
      <interactive desmos="fxuhxkxksv"/>
    </p>
  </solution>
</exercise>


<exercise>
  <statement>
    <p>
      A company purchases a  truck depreciates according to the
formula

<me> V(t)=\frac{60000}{1+0.5t+0.1t^2}</me> where <m>V</m> is measured in dollars and <m>t</m> is years after purchase.</p>
<p>
Find the rate the truck's value is changing in:
<ol>
  <li>Three years.</li>
  <li> Ten years.</li>
</ol>  

    </p>
  </statement>

<solution>
  <p>
    First note that <m>V(t)=60000(1+0.5t+0.1t^2)^{-1}</m>. So the truck's value changes according to:

    <md>
        <mrow>V'(t)\amp = \frac{d}{dt}[60000(1+0.5t+0.1t^2)^{-1}]</mrow>
         <mrow>\amp = 60000(-1)(1+0.5t+0.1t^2)^{-2}\frac{d}{dt}[1+0.5t+0.1t^2]</mrow>
         <mrow>\amp = 60000(-1)(1+0.5t+0.1t^2)^{-2}(0.5+0.2t)</mrow>
          <mrow>\amp = \frac{-30000-12000t}{(1+0.5t+0.1t^2)^{2}}</mrow>
      </md>.
Thus:
    <ol>
  <li> <m>N'(3)=\frac{-30000-12000(3)}{(1+0.5(3)+0.1(3)^2)^{2}}\approx -5709.34</m>.  So the truck is losing <m>\$5709.34</m> a year.

</li>
  <li> <m>N'(10)=\frac{-30000-12000(10)}{(1+0.5(10)+0.1(10)^2)^{2}}\approx -585.94</m>.  So the truck is losing <m>\$585.94</m> a year.

</li>
</ol>  

  
      We can see this:
      <interactive desmos="bdwnifm3dz"/>
    </p>
  </solution>
</exercise>


</subsection>

</section>