<section xml:id="Sec_RulesofDerivative">
  <title>Basic rules of the derivative</title>
  <introduction>
    <statement>
      <p>
        While there is a formal definition of a derivative, it is a somewhat cumbersome and computationally intense definition.  In this section, we begin introducing some properties of the derivative which simplify computation.
      </p>
    </statement>
  </introduction>
  <subsection>
  <title>Basic Rules</title>      
  
    <remark xml:id="RemarkLinear">
      <statement>
  <p>
    Given functions <m>f(x), g(x)</m> and constants <m>a,b</m> we have:
    <me>
      \frac{d}{dx}[a(f)x)+bg(x)]=af'(x)+bg'(x)
    </me>.
    Where <m>\frac{d}{dx}</m> means <q>to take the dertivative with respect to <m>x</m></q>.
  </p>
</statement>
</remark>
  <p>
    How do we know that?
    Well:
    <md>
      <mrow>\frac{d}{dx}[a(f)x)+bg(x)]\amp = \limit{h}{0}\frac{af(x+h)+bg(x+h)-(af(x)-bg(x))}{h}</mrow>
      <mrow>\amp = \limit{h}{0}\frac{af(x+h)-af(x)}{h}+\limit{h}{0}\frac{bg(x+h)-bg(x)}{h}</mrow>
      <mrow>\amp = a\limit{h}{0}\frac{f(x+h)-f(x)}{h}+b\limit{h}{0}\frac{g(x+h)-g(x)}{h}</mrow>
      <mrow>\amp = af'(x)+bg'(x)</mrow>
    </md>.
  </p>

</subsection>

<subsection>
  <title>Power Rule </title>
<p>
      We may have noticed a pattern with derivatives.
      But to illustrate it explicitly:
      <ul>
        <li>
          <p>
            The derivative of <m>f(x)=x^0</m>,
            it's the derivative of the constant function <m>f(x)=1</m>,
            and since its a horizontal line,
            it never has any slope and <m>f'(x)=0</m>.
          </p>
        </li>
        <li>
          <p>
            The derivative of <m>f(x)=x^1</m>,
            it's the derivative of the line <m>f(x)=x</m> which always has slope 1, so <m>f'(x)=1</m>.
          </p>
        </li>
        <li>
          <p>
            The derivative of <m>f(x)=x^2</m> is:
            <md>
              <mrow>\frac{d}{dx}[x^2]\amp = \limit{h}{0}\frac{f(x+h)-f(x)}{h}</mrow>
              <mrow>\amp = \limit{h}{0} \frac{(x+h)^2-x^2}{h}</mrow>
              <mrow>\amp = \limit{h}{0} \frac{x^2+2xh+h^2-x^2}{h}</mrow>
              <mrow>\amp = \limit{h}{0} \frac{(2x+h)h}{h}</mrow>
              <mrow>\amp = \limit{h}{0} 2x+h=2x</mrow>
            </md>.
          </p>
        </li>
        <li>
          <p>
            The derivative of <m>f(x)=x^3</m> is:
            <md>
              <mrow>\frac{d}{dx}[x^3]\amp = \limit{h}{0}\frac{f(x+h)-f(x)}{h}</mrow>
              <mrow>\amp = \limit{h}{0} \frac{(x+h)^3-x^3}{h}</mrow>
              <mrow>\amp = \limit{h}{0} \frac{x^3+3x^2h+3xh^2+h^3-x^3}{h}</mrow>
              <mrow>\amp = \limit{h}{0} \frac{(3x^2+3xh+h^2)h}{h}</mrow>
              <mrow>\amp = \limit{h}{0} 3x^2+3xh+h^2=3x^2</mrow>
            </md>.
          </p>
        </li>
      </ul>
    </p>
    <p>
      To generalize this, we have a rule of differentiation:
      <term> power rule</term>.</p>
    <remark>
      <statement>
      <p>
      <m>\frac{d}{dx}[x^n]=nx^{n-1}</m>.
    </p>
  </statement>
</remark>
    <p>
      To verify:
      <ul>
        <li>
          <p>
            <m>\frac{d}{dx}[x^0]=0x^{0-1}=0</m>.
          </p>
        </li>
        <li>
          <p>
            <m>\frac{d}{dx}[x^1]=1x^{1-1}=1</m>.
          </p>
        </li>
        <li>
          <p>
            <m>\frac{d}{dx}[x^2]=2x^{2-1}=2x</m>.
          </p>
        </li>
        <li>
          <p>
            <m>\frac{d}{dx}[x^3]=3x^{3-1}=3x^2</m>.
          </p>
        </li>
      </ul>
    </p>
    <p>
      What's fascinating is that this rule applies to <term> all</term>
      powers, not just integer powers.
    </p>

<remark xml:id="RemarkPower">
      <statement>
  <p>
    By rewriting functions into their power rule form:
    <ul>
      <li><m>\frac{d}{dx}[\frac{1}{x^n}]=\frac{d}{dx}[x^{-n}]=-nx^{-n+1}=\frac{-n}{x^{-n+1}}</m>.</li>
      <li><m>\frac{d}{dx}[\sqrt[n]{x}]=\frac{d}{dx}[x^{1/n}]=-\frac{1}{n}x^{\frac{1-n}{n}}=\frac{1}{\sqrt[n]{x^{n-1}}}</m>.</li>
    </ul>  
  </p>
</statement>
</remark>


<example>
  <title>Computing the derivative of a polynomial</title>
  <statement>
    <p>
      Find the derivative of <m>f(x)=x^4-2x^2+7x-3</m>.
    </p>
  </statement>
  <solution>
    <p>
    By <xref ref="RemarkPower"/> and <xref ref="RemarkLinear"/> we have:
      <md>
        <mrow>f'(x)\amp = \frac{d}{dx}[x^4-2x^2+7x-3]</mrow>
        <mrow>\amp = \frac{d}{dx}[x^4-2x^2+7x^1-3x^0]</mrow>
        <mrow>\amp = 4x^3-2(2x^1)+7(1x^0)-3(0x^{-1})</mrow>
        <mrow>\amp = 4x^3-4x+7</mrow>
      </md>.
    We can see this below:
    <interactive desmos="f7rllemfvp"  />
      </p>
    </solution>
</example> 


<example>
  <title>Computing the derivative more generally</title>
  <statement>
    <p>
      Find the derivative of <m>g(x)=\sqrt{4x}+\frac{3}{x}-\frac{2}{x^2}</m>.
    </p>
  </statement>
  <solution>
    <p>
    By <xref ref="RemarkPower"/> and <xref ref="RemarkLinear"/> we have:
      <md>
        <mrow>g'(x)\amp = \frac{d}{dx}[\sqrt{4x}+\frac{3}{x}-\frac{2}{x^2}]</mrow>
        <mrow>\amp = \frac{d}{dx}[2x^{1/2}+3x^{-1}-2x^{-2}]</mrow>
        <mrow>\amp = 2(1/2)x^{-1/2}+3(-1x^{-2})-2(2x^{-3})</mrow>
        <mrow>\amp = x^{-1/2}-3x^{-2}+4x^{-3}</mrow>
        <mrow>\amp = \frac{1}{\sqrt{x}}-\frac{3}{x^2}+\frac{4}{x^3}</mrow>
      </md>.
    We can see this below:
    <interactive desmos="fi1nqzbrpf"  />
      </p>
    </solution>
</example>  



<exercise>
  <title>Marginal Cost, Revenue and Profit</title>
  <statement>
    <p>
      An analyst has found that a companyâ€™s costs and revenues
in dollars for one product are given by
<me>C(x)=2x, R(x)=6x-\frac{x^2}{100}</me>
respectively, where <m>x</m> is the number of items produced.

    <ol>
      <li>Find the marginal cost function (<m>R'(x)</m> ).</li>
      <li> Find the marginal revenue function (<m>C'(x)</m> ).</li>
      <li> Using the fact that profit is the difference between revenue and costs, find the marginal profit function.</li>
      <li> What value of <m>x</m> makes marginal profit equal 0?</li>
      <li>Find the profit when the marginal profit is 0.</li>
    </ol>
    </p>
  </statement>
  <solution>
    <p>
    We have:
      <ol>
      <li> <m>C'(x)=\frac{d}{dx}[2x]=2</m>.  So <m>\$2</m> per product </li>
      <li> <m>R'(x)=\frac{d}{dx}[6x-\frac{x^2}{100}]=6-\frac{x}{50}</m>.  So <m>\$(6-\frac{x}{50})</m> per product </li>
      <li> <m>P(x)=R(x)-C(x)=6x-\frac{x^2}{100}-2x=4x-\frac{x^2}{100}.</m>.</li>
      <li> Since <m>P'(x)=\frac{d}{dx}[4x-\frac{x^2}{100}]=4-\frac{x}{50} </m>, we note that this is zero when:
      <md>
        <mrow>4-\frac{x}{50}\amp =0</mrow>
        <mrow>4\amp= \frac{x}{50}</mrow>
        <mrow>x\amp=200</mrow>
      </md>.
      So marginal profit is 0 when 200 units of the product are produced.
    </li>
      <li>We have <m>P(200)=4(200)-\frac{200^2}{100} =\$400</m>.</li>
    </ol>
    We can see this below:
    <interactive desmos="zmm7wvosxu"  />
      </p>
    </solution>
</exercise>  



<exercise>
  <title>Marginal Revenue</title>
  <statement>
    <p>
     If the price in dollars of a product is given by <me>p(q)=\frac{500}{q^2}+800</me> where <m>q</m> represents the demand for the product, find the marginal
revenue when the demand is 4.
    </p>
  </statement>
  <solution>
    <p>
    We  note that revenue is price times quantity demanded so <m>R(q)=p(q)q=(\frac{500}{q^2}+800)q=\frac{500}{q}+800q.</m>  From here we can find the marginal revenue: <m>R'(q)=\frac{d}{dq}[\frac{500}{q}+800q]=\frac{d}{dq}[500q^{-1}+800q]=-500q^{-2}+800=\frac{-500}{q^2}+800</m>.</p>
    <p>
    Thus, when demand is 4, the marginal revenue is <m>R'(4)=\frac{-500}{4^2}+800=\$768.75</m> per unit. We can see this below:
    <interactive desmos="l5leccci0i"  />
      </p>
    </solution>
</exercise>   


<exercise>
  <title>Blood Sugar levels</title>
  <statement>
    <p>
    Insulin affects the glucose, or blood sugar,
level of some diabetics according to the function <me>G(x)=-0.2x^2 +450,</me>
where <m>G(x)</m> is the blood sugar level 1 hour after <m>x</m> units of
insulin are injected. (This mathematical model is only approximate,
and it is valid only for values of x less than about 40.)
</p>
<p>
<ol>
<li>Find the blood sugar level after 10 units of insulin are injected.</li>
<li>Find the blood sugar level after 25 units of insulin are injected.</li>
<li>Find the rate of change of blood sugar level after 10 units of insulin are injected.</li>
<li>Find the rate of change of blood sugar level after 25 units of insulin are injected.</li>
</ol>
    </p>
  </statement>
  <solution>
    <p>
    We  note that <m>G'(x)=\frac{d}{dx}[-0.2x^2 +450]=-0.4x </m>.
    <ol>
<li><m>G(10)=-0.2(10)^2 +450=430.</m></li>
<li><m>G(25)=-0.2(25)^2 +450=325.</m></li>
<li><m>G'(10)=-0.4(10)=-4.</m></li>
<li><m>G'(25)=-0.4(25) =-10.</m></li>

</ol>


   We can see this below:
    <interactive desmos="2u2ktccdm7"  />
      </p>
    </solution>
</exercise> 










</subsection>
</section>